bigodafny/solutions/307/307_14.dfy
@@ -17,5 +17,40 @@ import opened Prelude
 
 method Solve(n: int, s: string) returns (output: string)
 {
-  output := ""; // TODO: translate the Python above
+  var cur := s;
+  var i := 100;
+  while i >= 1
+    decreases i
+  {
+    var pat := "o" + RepeatGo(i);
+    cur := ReplaceAll(cur, pat, "***");
+    i := i - 1;
+  }
+  output := cur + "\n";
+}
+
+function RepeatGo(i: int): string
+  requires i >= 0
+  decreases i
+{
+  if i == 0 then "" else "go" + RepeatGo(i - 1)
+}
+
+method ReplaceAll(s: string, pat: string, rep: string) returns (res: string)
+  requires |pat| > 0
+{
+  var parts: seq<string> := [];
+  var i := 0;
+  while i < |s|
+    decreases |s| - i
+  {
+    if i + |pat| <= |s| && s[i..i+|pat|] == pat {
+      parts := parts + [rep];
+      i := i + |pat|;
+    } else {
+      parts := parts + [[s[i]]];
+      i := i + 1;
+    }
+  }
+  res := Join(parts, "");
 }
