bigodafny/solutions/499/499_82.dfy
@@ -24,5 +24,24 @@ import opened Prelude
 
 method Solve(n: int, a_list: seq<int>) returns (output: string)
 {
-  output := ""; // TODO: translate the Python above
+  var a := SortInts(a_list);
+  var ans := 0;
+  var i := 0;
+  while i < n - 1
+    decreases n - 1 - i
+  {
+    var opt1 := Abs82(-1 - a[i+1]) + Abs82(-1 - a[i]);
+    var opt2 := Abs82(1 - a[i+1]) + Abs82(1 - a[i]);
+    ans := ans + (if opt1 < opt2 then opt1 else opt2);
+    i := i + 2;
+  }
+  if n % 2 == 1 {
+    ans := ans + Abs82(1 - a[n-1]);
+  }
+  output := IntToString(ans) + "\n";
+}
+
+function Abs82(x: int): int
+{
+  if x < 0 then -x else x
 }
