bigodafny/solutions/514/514_140.dfy
@@ -30,5 +30,47 @@ import opened Prelude
 
 method Solve(n: int, total_score: int, scores: seq<int>) returns (output: string)
 {
-  output := ""; // TODO: translate the Python above
+  var l := total_score;
+  var p := scores;
+  var idx := 0;
+  var ratios: seq<(real, int)> := [];
+  while idx < n
+    decreases n - idx
+  {
+    var r := (p[idx] as real) / (Pow2_140(idx) as real);
+    ratios := ratios + [(r, idx + 1)];
+    idx := idx + 1;
+  }
+  var d := Sort(ratios, (x: (real, int), y: (real, int)) => x.0 < y.0);
+  var res := 1000000000000000000;
+  var q := l;
+  var curres := 0;
+  var k := 0;
+  var doneFlag := false;
+  while k < |d| && !doneFlag
+    decreases |d| - k
+  {
+    var idxPos := d[k].1;
+    if idxPos == 1 {
+      curres := curres + p[idxPos - 1] * q;
+      res := if curres < res then curres else res;
+      doneFlag := true;
+    } else {
+      var pw := Pow2_140(idxPos - 1);
+      var curb := q / pw;
+      curres := curres + curb * p[idxPos - 1];
+      var cand := curres + p[idxPos - 1];
+      res := if cand < res then cand else res;
+      q := q % pw;
+    }
+    k := k + 1;
+  }
+  output := IntToString(res) + "\n";
+}
+
+function Pow2_140(e: int): int
+  requires e >= 0
+  decreases e
+{
+  if e == 0 then 1 else 2 * Pow2_140(e - 1)
 }
