bigodafny/solutions/514/514_90.dfy
@@ -24,5 +24,79 @@ import opened Prelude
 
 method Solve(n: int, total_score: int, scores: seq<int>) returns (output: string)
 {
-  output := ""; // TODO: translate the Python above
+  var x := total_score;
+  var a := scores;
+  var i := 1;
+  while i < n
+    decreases n - i
+  {
+    var cand := 2 * a[i-1];
+    a := a[i := if a[i] < cand then a[i] else cand];
+    i := i + 1;
+  }
+  var bx := RepeatChar90('0', n) + IntToBinary90(x);
+  var ans := FCost90(bx, n, a);
+  var j := 0;
+  while j < |bx|
+    decreases |bx| - j
+  {
+    if bx[j] == '0' {
+      var candStr := bx[..j] + "1" + RepeatChar90('0', |bx| - j - 1);
+      var candVal := FCost90(candStr, n, a);
+      ans := if candVal < ans then candVal else ans;
+    }
+    j := j + 1;
+  }
+  output := IntToString(ans) + "\n";
+}
+
+function Pow2_90(e: int): int
+  requires e >= 0
+  decreases e
+{
+  if e == 0 then 1 else 2 * Pow2_90(e - 1)
+}
+
+function ParseBinary90(bs: string): int
+  decreases |bs|
+{
+  if |bs| == 0 then 0
+  else ParseBinary90(bs[..|bs|-1]) * 2 + (if bs[|bs|-1] == '1' then 1 else 0)
+}
+
+function RepeatChar90(c: char, k: int): string
+  requires k >= 0
+  decreases k
+{
+  if k == 0 then "" else [c] + RepeatChar90(c, k - 1)
+}
+
+function IntToBinaryPos90(x: int): string
+  requires x >= 1
+  decreases x
+{
+  if x == 1 then "1"
+  else IntToBinaryPos90(x / 2) + [if x % 2 == 1 then '1' else '0']
+}
+
+function IntToBinary90(x: int): string
+  requires x >= 0
+{
+  if x == 0 then "0" else IntToBinaryPos90(x)
+}
+
+function LowSum90(bs: string, a: seq<int>, i: int, limit: int): int
+  decreases limit - i
+{
+  if i >= limit || i < 0 || limit > |bs| || limit > |a| then 0
+  else (if bs[|bs| - 1 - i] == '1' then a[i] else 0) + LowSum90(bs, a, i + 1, limit)
+}
+
+function FCost90(bs: string, n: int, a: seq<int>): int
+  requires n >= 1
+  requires |a| == n
+{
+  var L := |bs|;
+  var lim := if n - 1 <= L then n - 1 else L;
+  ParseBinary90(bs) / Pow2_90(n - 1) * a[n-1] + LowSum90(bs, a, 0, lim)
 }
