bigodafny/solutions/531/531_3456.dfy
@@ -20,5 +20,40 @@ import opened Prelude
 
 method Solve(matrix: seq<seq<int>>) returns (output: string)
 {
-  output := ""; // TODO: translate the Python above
+  var row := 1;
+  var col := 1;
+  var i := 0;
+  var found := false;
+  while i < 5 && !found
+    decreases 5 - i
+  {
+    var r := matrix[i];
+    if AllSame3456(r) {
+      row := row + 1;
+    } else {
+      col := IndexOf1From3456(r, 0) + 1;
+      found := true;
+    }
+    i := i + 1;
+  }
+  output := IntToString(Abs3456(3 - row) + Abs3456(3 - col)) + "\n";
+}
+
+function AllSame3456(r: seq<int>): bool
+{
+  forall k :: 0 <= k < |r| ==> r[k] == r[0]
+}
+
+function IndexOf1From3456(r: seq<int>, i: int): int
+  requires 0 <= i <= |r|
+  decreases |r| - i
+{
+  if i >= |r| then -1
+  else if r[i] == 1 then i
+  else IndexOf1From3456(r, i + 1)
+}
+
+function Abs3456(x: int): int
+{
+  if x < 0 then -x else x
 }
