bigodafny/solutions/531/531_3499.dfy
@@ -53,5 +53,31 @@ import opened Prelude
 
 method Solve(matrix: seq<seq<int>>) returns (output: string)
 {
-  output := ""; // TODO: translate the Python above
+  var result := 0;
+  var i := 0;
+  while i < 5
+    decreases 5 - i
+  {
+    var r := matrix[i];
+    var idx := IndexOf1From3499(r, 0);
+    if idx >= 0 {
+      result := Abs3499(2 - i) + Abs3499(2 - idx);
+    }
+    i := i + 1;
+  }
+  output := IntToString(result) + "\n";
+}
+
+function IndexOf1From3499(r: seq<int>, i: int): int
+  requires 0 <= i <= |r|
+  decreases |r| - i
+{
+  if i >= |r| then -1
+  else if r[i] == 1 then i
+  else IndexOf1From3499(r, i + 1)
+}
+
+function Abs3499(x: int): int
+{
+  if x < 0 then -x else x
 }
